theories/SetModel/CwF_library.v
@@ -3,62 +3,122 @@ Require Import ZF_axioms.
 Require Import ZF_library.
 Require Import CwF.
 
+(* Elements of 𝕌 are also elements of 𝕍 *)
+
+Lemma 𝕌_incl_𝕍 {n : nat} : 𝕌 n ⊂ 𝕍 n.
+Proof.
+  intros x Hx. refine (transpS (fun X => X ∈ 𝕍 n) (sym (setPairη Hx)) _). apply setMkPair_sorting.
+  - now apply setFstPair_typing.
+  - set (y := setSndPair (𝕍 n) (ω × 𝕍 n) x). assert (y ∈ ω × 𝕍 n) as Hy. { now apply setSndPair_typing. }
+    clearbody y. clear x Hx. refine (transpS (fun X => X ∈ 𝕍 n) (sym (setPairη Hy)) _). apply setMkPair_sorting.
+    + eapply ZFuniv_trans. now apply setFstPair_typing. apply ZFuniv_uncountable.
+    + now apply setSndPair_typing.
+Qed.
+
 (* Defining terms and types using higher-order stuff *)
 
-Definition HO_Ty (n : nat) (Γ : ZFSet) (f : ZFSet -> ZFSet) := relToGraph Γ (𝕍 n × (ω × 𝕍 n)) (HO_rel f).
-Definition HO_Tm (n : nat) (Γ : ZFSet) (f : ZFSet -> ZFSet) := relToGraph Γ (𝕍 n) (HO_rel f).
+Definition HO_to_cwfTy (n : nat) (Γ : ZFSet) (f : ZFSet -> ZFSet) :=
+  relToGraph Γ (𝕌 n) (HO_rel f).
 
-Lemma HO_Tm_pretyping {n : nat} {Γ : ZFSet} {f : ZFSet -> ZFSet} (Hf : ∀ γ ∈ Γ, f γ ∈ 𝕍 n) : HO_Tm n Γ f ∈ Γ ⇒ 𝕍 n.
+Definition HO_to_cwfTm (n : nat) (Γ : ZFSet) (f : ZFSet -> ZFSet) :=
+  relToGraph Γ (𝕍 n) (HO_rel f).
+
+Definition cwfTy_to_HO (n : nat) (Γ A : ZFSet) :=
+  fun γ => setAppArr Γ (𝕌 n) A γ.
+
+Definition cwfTy_to_HO2 (n : nat) (Γ A B : ZFSet) :=
+  fun γ a => setAppArr (ctxExt n Γ A) (𝕌 n) B ⟨ γ ; a ⟩.
+
+Lemma cwfTy_to_HO_typing {n : nat} {Γ A : ZFSet} (HA : A ∈ cwfTy n Γ) : ∀ γ ∈ Γ, cwfTy_to_HO n Γ A γ ∈ 𝕌 n.
+Proof.
+  intros γ Hγ. now apply setAppArr_typing.
+Qed.
+
+Lemma cwfTy_to_HO2_typing {n : nat} {Γ A B : ZFSet} (HA : A ∈ cwfTy n Γ) (HB : B ∈ cwfTy n (ctxExt n Γ A)) :
+  ∀ γ ∈ Γ, ∀ a ∈ 𝕌el n (cwfTy_to_HO n Γ A γ), cwfTy_to_HO2 n Γ A B γ a ∈ 𝕌 n.
+Proof.
+  intros γ Hγ a Ha. apply setAppArr_typing. assumption.
+  apply setMkSigma_typing.
+  - clear γ Hγ a Ha. intros γ Hγ. now apply cwfTy_to_depSet_typing.
+  - assumption.
+  - assumption.
+Qed.
+
+Lemma HO_to_cwfTy_sorting (n : nat) {A : ZFSet} {B : ZFSet -> ZFSet} (HA : A ∈ 𝕍 n) (HB : ∀ a ∈ A, B a ∈ 𝕌 n)
+  : HO_to_cwfTy n A B ∈ 𝕍 n.
+Proof.
+  assert (relToGraph A (𝕌 n) (HO_rel B) ∈ A ⇒ 𝕌 n).
+  { apply relToGraph_typing. now apply HO_rel_typing. }
+  assert (A ⇒ 𝕌 n ⊂ 𝕍 n) as H1.
+  { apply setArr_big_typing. assumption. apply 𝕌_incl_𝕍. }
+  now apply H1.
+Qed.
+
+Lemma HO_to_cwfTm_pretyping {n : nat} {Γ : ZFSet} {f : ZFSet -> ZFSet} (Hf : ∀ γ ∈ Γ, f γ ∈ 𝕍 n) :
+  HO_to_cwfTm n Γ f ∈ Γ ⇒ 𝕍 n.
 Proof.
   apply relToGraph_typing. now apply HO_rel_typing.
 Qed.
-  
-Lemma cwfTy_to_depSet_HO_Ty {n : nat} {Γ γ : ZFSet} {f : ZFSet -> ZFSet} (Hf : ∀ γ ∈ Γ, f γ ∈ 𝕍 n × (ω × 𝕍 n)) (Hγ : γ ∈ Γ) :
-  cwfTy_to_depSet n Γ (HO_Ty n Γ f) γ ≡ setFstPair (𝕍 n) (ω × 𝕍 n) (f γ).
+
+Lemma setAppArr_HO_to_cwfTm {n : nat} {Γ γ : ZFSet} {f : ZFSet -> ZFSet} (Hf : ∀ γ ∈ Γ, f γ ∈ 𝕍 n) (Hγ : γ ∈ Γ) : 
+  setAppArr Γ (𝕍 n) (HO_to_cwfTm n Γ f) γ ≡ f γ.
+Proof.
+  now apply setAppArr_HO.
+Qed.
+
+Lemma HO_to_cwfTy_to_depSet {n : nat} {Γ γ : ZFSet} {f : ZFSet -> ZFSet} (Hf : ∀ γ ∈ Γ, f γ ∈ 𝕌 n) (Hγ : γ ∈ Γ) :
+  cwfTy_to_depSet n Γ (HO_to_cwfTy n Γ f) γ ≡ 𝕌el n (f γ).
 Proof.
   refine (fequal (setFstPair _ _) _).
   now apply setAppArr_HO.
 Qed. 
 
-Lemma setAppArr_HO_Tm {n : nat} {Γ γ : ZFSet} {f : ZFSet -> ZFSet} (Hf : ∀ γ ∈ Γ, f γ ∈ 𝕍 n) (Hγ : γ ∈ Γ) : 
-  setAppArr Γ (𝕍 n) (HO_Tm n Γ f) γ ≡ f γ.
-Proof.
-  now apply setAppArr_HO.
-Qed.
-
 Lemma setAppArr_Tm_typing {n : nat} {Γ t : ZFSet} {A : ZFSet -> ZFSet}
-  (HA : ∀ γ ∈ Γ, A γ ∈ 𝕍 n × (ω × 𝕍 n)) (Ht : t ∈ Γ ⇒ 𝕍 n) :
-  (∀ γ ∈ Γ, setAppArr Γ (𝕍 n) t γ ∈ setFstPair (𝕍 n) (ω × 𝕍 n) (A γ)) -> (t ∈ cwfTm n Γ (HO_Ty n Γ A)).
+  (HA : ∀ γ ∈ Γ, A γ ∈ 𝕌 n) (Ht : t ∈ Γ ⇒ 𝕍 n) :
+  (∀ γ ∈ Γ, setAppArr Γ (𝕍 n) t γ ∈ 𝕌el n (A γ)) -> (t ∈ cwfTm n Γ (HO_to_cwfTy n Γ A)).
 Proof.
   intro Ht'. apply ZFincomp. split ; try assumption.
   intros γ Hγ. refine (transpS (fun x => _ ∈ x) _ (Ht' γ Hγ)).
-  symmetry. now apply cwfTy_to_depSet_HO_Ty.
+  symmetry. now apply HO_to_cwfTy_to_depSet.
 Qed.
 
 Lemma setAppArr_Tm_detyping {n : nat} {Γ t : ZFSet} {A : ZFSet -> ZFSet}
-  (HA : ∀ γ ∈ Γ, A γ ∈ 𝕍 n × (ω × 𝕍 n)) :
-  (t ∈ cwfTm n Γ (HO_Ty n Γ A)) -> ∀ γ ∈ Γ, setAppArr Γ (𝕍 n) t γ ∈ setFstPair (𝕍 n) (ω × 𝕍 n) (A γ).
+  (HA : ∀ γ ∈ Γ, A γ ∈ 𝕌 n) :
+  (t ∈ cwfTm n Γ (HO_to_cwfTy n Γ A)) -> ∀ γ ∈ Γ, setAppArr Γ (𝕍 n) t γ ∈ 𝕌el n (A γ).
 Proof.
   intros Ht' γ Hγ. apply ZFincomp in Ht'. destruct Ht' as [ _ Ht' ].
   refine (transpS (fun x => _ ∈ x) _ (Ht' γ Hγ)).
-  now apply cwfTy_to_depSet_HO_Ty.
+  now apply HO_to_cwfTy_to_depSet.
 Qed.
 
-Lemma HO_Tm_typing {n : nat} {Γ : ZFSet} {f A : ZFSet -> ZFSet}
-  (HA : ∀ γ ∈ Γ, A γ ∈ 𝕍 n × (ω × 𝕍 n)) :
-  (∀ γ ∈ Γ, f γ ∈ setFstPair (𝕍 n) (ω × 𝕍 n) (A γ)) -> (HO_Tm n Γ f ∈ cwfTm n Γ (HO_Ty n Γ A)).
+Lemma HO_to_cwfTm_typing {n : nat} {Γ : ZFSet} {f A : ZFSet -> ZFSet}
+  (HA : ∀ γ ∈ Γ, A γ ∈ 𝕌 n) :
+  (∀ γ ∈ Γ, f γ ∈ 𝕌el n (A γ)) -> (HO_to_cwfTm n Γ f ∈ cwfTm n Γ (HO_to_cwfTy n Γ A)).
 Proof.
   intro H. assert (∀ γ ∈ Γ, f γ ∈ 𝕍 n) as Hf.
   { intros γ Hγ. eapply ZFuniv_trans. now apply H. apply setFstPair_typing. now apply HA. }
-  eapply (setAppArr_Tm_typing HA (HO_Tm_pretyping Hf)).
+  eapply (setAppArr_Tm_typing HA (HO_to_cwfTm_pretyping Hf)).
   intros γ Hγ. refine (transpS (fun x => x ∈ _) _ (H γ Hγ)).
-  symmetry. now apply setAppArr_HO_Tm.
+  symmetry. now apply setAppArr_HO_to_cwfTm.
 Qed.
 
-Lemma HO_Tm_detyping {n : nat} {Γ : ZFSet} {f A : ZFSet -> ZFSet}
-  (HA : ∀ γ ∈ Γ, A γ ∈ 𝕍 n × (ω × 𝕍 n)) (Hf : ∀ γ ∈ Γ, f γ ∈ 𝕍 n) :
-  (HO_Tm n Γ f ∈ cwfTm n Γ (HO_Ty n Γ A)) -> (∀ γ ∈ Γ, f γ ∈ setFstPair (𝕍 n) (ω × 𝕍 n) (A γ)).
+Lemma HO_to_cwfTm_detyping {n : nat} {Γ : ZFSet} {f A : ZFSet -> ZFSet}
+  (HA : ∀ γ ∈ Γ, A γ ∈ 𝕌 n) (Hf : ∀ γ ∈ Γ, f γ ∈ 𝕍 n) :
+  (HO_to_cwfTm n Γ f ∈ cwfTm n Γ (HO_to_cwfTy n Γ A)) -> (∀ γ ∈ Γ, f γ ∈ 𝕌el n (A γ)).
 Proof.
   intros H γ Hγ. eapply (setAppArr_Tm_detyping HA) in H.
-  refine (transpS (fun x => x ∈ _) _ H). now apply setAppArr_HO_Tm. assumption.
+  refine (transpS (fun x => x ∈ _) _ H). now apply setAppArr_HO_to_cwfTm. assumption.
+Qed.
+
+(* Telescopes (useful for labels) *)
+
+Definition typeTelescope2 (n : nat) (Γ : ZFSet) (A : ZFSet -> ZFSet) (B : ZFSet -> ZFSet -> ZFSet) :=
+  fun γ => ⟨ A γ ; HO_to_cwfTy n (𝕌el n (A γ)) (B γ) ⟩.
+
+Lemma typeTelescope2_typing (n : nat) {Γ : ZFSet} {A : ZFSet -> ZFSet} {B : ZFSet -> ZFSet -> ZFSet}
+  (HA : ∀ γ ∈ Γ, A γ ∈ 𝕌 n) (HB : ∀ γ ∈ Γ, ∀ a ∈ 𝕌el n (A γ), B γ a ∈ 𝕌 n) : ∀ γ ∈ Γ, typeTelescope2 n Γ A B γ ∈ 𝕍 n.
+Proof.
+  intros γ Hγ. cbn. unfold typeTelescope2. apply setMkPair_sorting.
+  - apply 𝕌_incl_𝕍. now apply HA.
+  - apply HO_to_cwfTy_sorting. apply 𝕌el_typing. now apply HA. now apply HB.
 Qed.
