theories/SetModel/CwF_nat.v
@@ -8,16 +8,16 @@ Require Import CwF_library.
 
 Definition natTy_HO : ZFSet -> ZFSet := fun _ => ⟨ ω ; ⟨ ∅ ; ∅ ⟩ ⟩.
 
-Definition natTy (n : nat) (Γ : ZFSet) := HO_Ty n Γ natTy_HO. 
+Definition natTy (n : nat) (Γ : ZFSet) := HO_to_cwfTy n Γ natTy_HO. 
 
-Lemma setFstPair_natTy {n : nat} {γ : ZFSet} : setFstPair (𝕍 n) (ω × 𝕍 n) (natTy_HO γ) ≡ ω.
+Lemma el_natTy {n : nat} {γ : ZFSet} : 𝕌el n (natTy_HO γ) ≡ ω.
 Proof.
   apply setPairβ1.
   + apply ZFuniv_uncountable.
   + apply setMkPair_typing. apply zero_typing. apply empty_in_univ.
 Qed.
 
-Lemma natTy_HO_typing (n : nat) {γ : ZFSet} : natTy_HO γ ∈ 𝕍 n × (ω × 𝕍 n).
+Lemma natTy_HO_typing (n : nat) {γ : ZFSet} : natTy_HO γ ∈ 𝕌 n.
 Proof.
   apply setMkPair_typing.
   - now apply ZFuniv_uncountable.
@@ -36,18 +36,18 @@ Qed.
 
 Definition zeroTm_HO : ZFSet -> ZFSet := fun _ => ∅.
 
-Definition zeroTm (n : nat) (Γ : ZFSet) := HO_Tm n Γ zeroTm_HO.
+Definition zeroTm (n : nat) (Γ : ZFSet) := HO_to_cwfTm n Γ zeroTm_HO.
 
-Lemma zeroTm_HO_typing (n : nat) {γ : ZFSet} : zeroTm_HO γ ∈ setFstPair (𝕍 n) (ω × 𝕍 n) (natTy_HO γ).
+Lemma zeroTm_HO_typing (n : nat) {γ : ZFSet} : zeroTm_HO γ ∈ 𝕌el n (natTy_HO γ).
 Proof.
   refine (transpS (fun x => _ ∈ x) _ _).
-  - symmetry. apply setFstPair_natTy. 
+  - symmetry. apply el_natTy. 
   - apply zero_typing.
 Qed.
 
 Lemma cwfZero {n : nat} (Γ : ZFSet) : zeroTm n Γ ∈ cwfTm n Γ (natTy n Γ).
 Proof.
-  apply HO_Tm_typing.
+  apply HO_to_cwfTm_typing.
   - intros. apply natTy_HO_typing.
   - intros γ Hγ. apply zeroTm_HO_typing.
 Qed.
@@ -58,16 +58,16 @@ Definition sucTm_HO (n : nat) (Γ : ZFSet) (t : ZFSet) : ZFSet -> ZFSet :=
   fun γ => ZFsuc (setAppArr Γ (𝕍 n) t γ).
 
 Definition sucTm (n : nat) (Γ : ZFSet) (t : ZFSet) :=
-  HO_Tm n Γ (sucTm_HO n Γ t).
+  HO_to_cwfTm n Γ (sucTm_HO n Γ t).
 
 Lemma sucTm_HO_typing {n : nat} {Γ t γ : ZFSet} (Ht : t ∈ cwfTm n Γ (natTy n Γ)) (Hγ : γ ∈ Γ) :
-  sucTm_HO n Γ t γ ∈ setFstPair (𝕍 n) (ω × 𝕍 n) (natTy_HO γ).
+  sucTm_HO n Γ t γ ∈ 𝕌el n (natTy_HO γ).
 Proof.
   refine (transpS (fun x => _ ∈ x) _ _).
-  { symmetry. apply setFstPair_natTy. }
+  { symmetry. apply el_natTy. }
   apply suc_typing.
   refine (transpS (fun x => _ ∈ x) _ _).
-  { apply (@setFstPair_natTy n γ). }
+  { apply (@el_natTy n γ). }
   apply setAppArr_Tm_detyping ; try assumption.
   intros ; apply natTy_HO_typing.
 Qed.
@@ -75,7 +75,7 @@ Qed.
 Lemma cwfSuc {n : nat} {Γ t : ZFSet} (Ht : t ∈ cwfTm n Γ (natTy n Γ)) :
   sucTm n Γ t ∈ cwfTm n Γ (natTy n Γ).
 Proof.
-  apply HO_Tm_typing.
+  apply HO_to_cwfTm_typing.
   - intros. apply natTy_HO_typing.
   - intros γ Hγ. now apply sucTm_HO_typing.
 Qed.
