theories/SetModel/CwF_pi.v
@@ -1,0 +1,45 @@
+Require Import library.
+Require Import ZF_axioms.
+Require Import ZF_library.
+Require Import CwF.
+Require Import CwF_library.
+
+
+Definition piTy_HO (n : nat) (Γ : ZFSet) (A : ZFSet -> ZFSet) (B : ZFSet -> ZFSet -> ZFSet) : ZFSet -> ZFSet :=
+  fun γ => ⟨ setPi n (𝕌el n (A γ)) (fun a => 𝕌el n (B γ a))
+           ; ⟨ ZFone ; typeTelescope2 n Γ A B γ ⟩ ⟩.
+
+Definition piTy (n : nat) (Γ : ZFSet) (A : ZFSet) (B : ZFSet) : ZFSet :=
+  HO_to_cwfTy n Γ (piTy_HO n Γ (cwfTy_to_HO n Γ A) (cwfTy_to_HO2 n Γ A B)).
+
+Lemma piTy_HO_typing (n : nat) {Γ : ZFSet} {A : ZFSet -> ZFSet} {B : ZFSet -> ZFSet -> ZFSet}
+  (HA : ∀ γ ∈ Γ, A γ ∈ 𝕌 n) (HB : ∀ γ ∈ Γ, ∀ a ∈ 𝕌el n (A γ), B γ a ∈ 𝕌 n) : ∀ γ ∈ Γ, piTy_HO n Γ A B γ ∈ 𝕌 n.
+Proof.
+  intros γ Hγ. cbn. apply setMkPair_typing.
+  - apply setPi_typing.
+    + apply 𝕌el_typing. now apply HA.
+    + intros a Ha. apply 𝕌el_typing. now apply HB. 
+  - apply setMkPair_typing.
+    + apply one_typing.
+    + now apply typeTelescope2_typing.
+Qed.
+
+Lemma el_piTy {n : nat} {Γ γ : ZFSet} {A : ZFSet -> ZFSet} {B : ZFSet -> ZFSet -> ZFSet}
+  (HA : ∀ γ ∈ Γ, A γ ∈ 𝕌 n) (HB : ∀ γ ∈ Γ, ∀ a ∈ 𝕌el n (A γ), B γ a ∈ 𝕌 n) (Hγ : γ ∈ Γ) :
+  𝕌el n (piTy_HO n Γ A B γ) ≡ setPi n (𝕌el n (A γ)) (fun a => 𝕌el n (B γ a)).
+Proof.
+  apply setPairβ1.
+  - apply setPi_typing. apply 𝕌el_typing. now apply HA.
+    intros a Ha. apply 𝕌el_typing. now apply HB.
+  - apply setMkPair_typing.
+    + apply one_typing.
+    + now apply typeTelescope2_typing.
+Qed.
+
+Lemma cwfPi {n : nat} {Γ A B : ZFSet} (HA : A ∈ cwfTy n Γ) (HB : B ∈ cwfTy n (ctxExt n Γ A)) :
+  piTy n Γ A B ∈ cwfTy n Γ.
+Proof.
+  apply relToGraph_typing. apply HO_rel_typing. apply piTy_HO_typing.
+  - now apply cwfTy_to_HO_typing.
+  - now apply cwfTy_to_HO2_typing.
+Qed.
