theories/SetModel/ZF_axioms.v
@@ -90,4 +90,5 @@ Axiom ZFuniv_hierarchy : forall n, 𝕍 n ∈ 𝕍 (n+1).
 Axiom ZFuniv_trans : forall n x y, x ∈ y -> y ∈ 𝕍 n -> x ∈ 𝕍 n.
 Axiom ZFuniv_pair : forall n x y, x ∈ 𝕍 n -> y ∈ 𝕍 n -> { x ; y } ∈ 𝕍 n.
 Axiom ZFuniv_power : forall n x, x ∈ 𝕍 n -> 𝒫 x ∈ 𝕍 n.
-(* Axiom ZFuniv_union : forall n I (φ : ZFSet -> ZFSet -> SProp), *)
+Axiom ZFuniv_union : forall n I (φ : ZFSet -> ZFSet -> SProp), I ∈ 𝕍 n -> (∀ i ∈ I, ∃! x ∈ 𝕍 n, φ i x)
+                                                               -> ⋃ { x ϵ 𝕍 n ∣ ∃ i ∈ I, φ i x } ∈ 𝕍 n.
